examples/miniparse/MiniParse.Example.fsti
@@ -21,63 +21,12 @@ let f' : test -> Tot (bounded_u8 test_bound) = T.synth_by_tactic (fun () -> gen_
 
 let g' : bounded_u8 test_bound -> Tot test = T.synth_by_tactic (fun () -> invert_function  (`(test)) (`(bounded_u8 test_bound)) (`(op_Equality #(bounded_u8 test_bound))) (`(f')))
 
-let g'_injective: squash (synth_injective g') =
-  T.synth_by_tactic (fun () -> synth_injective_solve (`f'))
-
 let g'_inverse: squash (synth_inverse g' f') =
-  T.synth_by_tactic synth_inverse_solve
+  T.synth_by_tactic synth_inverse_forall_tenum_solve
+
+let g'_injective: squash (synth_inverse f' g') =
+  T.synth_by_tactic synth_inverse_forall_bounded_u8_solve
 
 let p : parser test = T.synth_by_tactic (fun () -> gen_enum_parser (`test))
 
 let q : parser32 p = T.synth_by_tactic (fun () -> gen_parser32 (`p))
-
-#reset-options
-
-// At this point, SMT is back on
-
-#set-options "--z3rlimit 32"
-
-let q' : parser32 p =
-  MiniParse.Impl.Combinators.parse32_synth (MiniParse.Spec.TEnum.parse_bounded_u8 4)
-  (fun x2 ->
-       MiniParse.Tac.Base.mk_if_t (MiniParse.Spec.TEnum.bounded_u8_eq 4
-             x2
-             (MiniParse.Spec.TEnum.mk_u8 0))
-         (fun _ -> TA)
-         (fun _ ->
-             MiniParse.Tac.Base.mk_if_t (MiniParse.Spec.TEnum.bounded_u8_eq 4
-                   x2
-                   (MiniParse.Spec.TEnum.mk_u8 1))
-               (fun _ -> TB)
-               (fun _ ->
-                   MiniParse.Tac.Base.mk_if_t (MiniParse.Spec.TEnum.bounded_u8_eq 4
-                         x2
-                         (MiniParse.Spec.TEnum.mk_u8 2))
-                     (fun _ -> TC)
-                     (fun _ -> TD))))
-   (fun x0 ->
-       (fun x2 ->
-           MiniParse.Tac.Base.mk_if_t (MiniParse.Spec.TEnum.bounded_u8_eq 4
-                 x2
-                 (MiniParse.Spec.TEnum.mk_u8 0))
-             (fun _ -> TA)
-             (fun _ ->
-                 MiniParse.Tac.Base.mk_if_t (MiniParse.Spec.TEnum.bounded_u8_eq 4
-                       x2
-                       (MiniParse.Spec.TEnum.mk_u8 1))
-                   (fun _ -> TB)
-                   (fun _ ->
-                       MiniParse.Tac.Base.mk_if_t (MiniParse.Spec.TEnum.bounded_u8_eq 4
-                             x2
-                             (MiniParse.Spec.TEnum.mk_u8 2))
-                         (fun _ -> TC)
-                         (fun _ -> TD)))) x0)
-   (MiniParse.Impl.Combinators.parse32_synth (MiniParse.Spec.Combinators.parse_filter MiniParse.Spec.Int.parse_u8
-           (fun x -> FStar.UInt8.v x < 4))
-       (fun x -> x <: MiniParse.Spec.TEnum.bounded_u8 4)
-       (fun x1 -> (fun x -> x <: MiniParse.Spec.TEnum.bounded_u8 4) x1)
-       (MiniParse.Impl.Combinators.parse32_filter MiniParse.Impl.Int.parse32_u8
-           (fun x -> FStar.UInt8.v x < 4)
-           (fun x2 -> (fun x -> FStar.UInt8.v x < 4) x2))
-       ())
-   ()
