examples/miniparse/MiniParse.Impl.TEnum.fst
@@ -12,7 +12,7 @@ let parse32_bounded_u8
   (b: nat)
 : Tot (parser32 (parse_bounded_u8 b)) =
   if b >= 256
-  then (fun input len -> parse32_synth parse32_u8 (fun x -> x <: bounded_u8 b) (fun x -> x <: bounded_u8 b) () input len)
+  then (fun input len -> parse32_synth parse32_u8 (fun x -> x <: bounded_u8 b) (fun x -> x <: bounded_u8 b) (fun x -> x) () input len)
   else
     [@inline_let]
     let b' = U8.uint_to_t b in
@@ -20,4 +20,5 @@ let parse32_bounded_u8
       (parse32_filter parse32_u8 (fun x -> U8.v x < b) (fun x -> x `U8.lt` b'))
       (fun x -> x <: bounded_u8 b)
       (fun x -> x <: bounded_u8 b)
+      (fun x -> x)
       ()
